Split ZX -> ZX, SemanticCore

ZX.v
@@ -1,855 +1,95 @@
-Require Import Coq.Vectors.Fin.
 Require Import externals.QuantumLib.Quantum.
 Require Import externals.QuantumLib.Proportional.
 Require Import externals.QuantumLib.VectorStates.
+From VyZX Require Export SemanticCore.
+
+(** Base constructions for the ZX calculus, lets us build every diagram inductively.
+    We have included some "unnecessary" objects because they are common and useful. *)
 
 Declare Scope ZX_scope.
-Local Open Scope ZX_scope.
+Delimit Scope ZX_scope with ZX.
+Open Scope ZX_scope.
 
-Local Open Scope R_scope.
 Inductive ZX : nat -> nat -> Type :=
   | Empty : ZX 0 0
-  | X_Spider nIn nOut (α : R) : ZX nIn nOut
-  | Z_Spider nIn nOut (α : R) : ZX nIn nOut
-  | Cap : ZX 0 2
-  | Cup : ZX 2 0
+  | Cap  : ZX 0 2
+  | Cup  : ZX 2 0
   | Swap : ZX 2 2
-  | Stack {nIn0 nIn1 nOut0 nOut1} (zx0 : ZX nIn0 nOut0) (zx1 : ZX nIn1 nOut1) :
-      ZX (nIn0 + nIn1) (nOut0 + nOut1)
-  | Compose {nIn nMid nOut} (zx0 : ZX nIn nMid) (zx1 : ZX nMid nOut) : ZX nIn nOut.
-Local Close Scope R_scope.
+  | Wire : ZX 1 1
+  | Box  : ZX 1 1
+  | X_Spider n m (α : R) : ZX n m
+  | Z_Spider n m (α : R) : ZX n m
+  | Stack {n_0 m_0 n_1 m_1} (zx0 : ZX n_0 m_0) (zx1 : ZX n_1 m_1) : ZX (n_0 + n_1) (m_0 + m_1)
+  | Compose {n_0 m n_1} (zx0 : ZX n_0 m) (zx1 : ZX m n_1) : ZX n_0 n_1.
 
-Notation "⦰" := Empty. (* \revemptyset *)
-Notation "⊂" := Cap. (* \subset *)
-Notation "⊃" := Cup. (* \supset *)
-Notation "⨉" := Swap. (* \bigtimes *)
-Infix "⟷" := Compose (left associativity, at level 40). (* \longleftrightarrow *)
-Infix "↕" := Stack (left associativity, at level 40). (* \updownarrow *)
+(* Notations for the ZX diagrams *)
+Notation "⦰" := Empty : ZX_scope. (* \revemptyset *)
+Notation "⊂" := Cap : ZX_scope. (* \subset *)
+Notation "⊃" := Cup : ZX_scope. (* \supset *)
+Notation "⨉" := Swap : ZX_scope. (* \bigtimes *)
+Notation "—" := Wire : ZX_scope. (* \emdash *)
+Notation "□" := Box : ZX_scope. (* \square *)
+Notation "A ⟷ B" := (Compose A B) (left associativity, at level 40) : ZX_scope. (* \longleftrightarrow *)
+Notation "A ↕ B" := (Stack A B) (left associativity, at level 40) : ZX_scope. (* \updownarrow *)
+Notation "'Z'" := Z_Spider (left associativity, at level 40) : ZX_scope.
+Notation "'X'" := X_Spider (left associativity, at level 40) : ZX_scope.
 
-(* TODO: Move into quantum lib *)
-Hint Rewrite Mscale_kron_dist_l Mscale_kron_dist_r Mscale_mult_dist_l Mscale_mult_dist_r Mscale_assoc : scalar_move_db.
+(** We provide two separate options for semantic functions, one based on sparse matrices
+    and one based on dirac notation. *)
 
-Definition Z_semantics (n m : nat) (α : R) : Matrix (2 ^ m) (2 ^ n) :=
-  fun x y =>
-  match x, y with
-  | 0, 0 => match n, m with
-                  | 0, 0 => C1 + Cexp α
-                  | _, _  => C1
-                  end
-  | _, _ => if ((x =? 2^m-1) && (y =? 2^n-1)) then Cexp α else C0
-  end.
-(* 
-bdestruct, takes a boolean equality and destructs it, reflects into context
-
-*)
-
-
-Lemma Z_semantics_transpose (n m : nat) (α : R) : (Z_semantics n m α) ⊤ = Z_semantics m n α.
-Proof.
-  unfold Z_semantics.
-  unfold transpose.
-  prep_matrix_equality.
-  destruct x, y.
-  - destruct n, m; reflexivity.
-  - destruct (S y =? 2^m - 1), (0 =? 2^n-1); reflexivity.
-  - destruct (0 =? 2^m - 1), (S x =? 2^n-1); reflexivity.
-  - destruct (S y =? 2^m-1), (S x =? 2^n-1); reflexivity.
-Qed.
-
-Lemma Z_semantics_adj (n m : nat) (α : R) : (Z_semantics n m α) † = Z_semantics m n (- α).
-Proof.
-  unfold Z_semantics.
-  unfold adjoint.
-  prep_matrix_equality.
-  destruct x,y. 
-  - destruct n,m; try lca.
-    rewrite Cconj_plus_distr.
-    rewrite Cexp_conj_neg.
-    lca.
-  - destruct (S y =? 2^m-1), (0=?2^n-1); try lca.
-    apply Cexp_conj_neg.
-  - destruct (0=?2^m-1),(S x=?2^n-1); try lca.
-    apply Cexp_conj_neg.
-  - destruct (S y=?2^m-1),(S x=?2^n-1); try lca.
-    apply Cexp_conj_neg.
-Qed.
-
-Lemma WF_Z_semantics {n m : nat} {α : R} : WF_Matrix (Z_semantics n m α).
-Proof.
-  unfold WF_Matrix; unfold Z_semantics.
-  assert ( GeqToEqb : forall (a b c : nat), b <= a  -> c < b -> a =? c = false ).
-  {
-    intros.
-    apply Nat.eqb_neq.
-    apply not_eq_sym.
-    apply (Nat.lt_neq c a).
-    apply (Nat.lt_le_trans c b a); assumption.
-  }
-  assert ( geq_symm : forall (a b : nat), a >= b -> b <= a).
-  {
-    induction a.
-    - intros.
-      inversion H.
-      reflexivity.
-    - intros.
-      inversion H; try reflexivity.
-      apply (Nat.le_le_succ_r _ _ H1).
-  }
-  assert ( expgt : forall a : nat, 2 ^ a - 1 < 2 ^ a).
-  {
-    intros.
-    induction a.
-    - constructor.
-    - simpl.
-      lia.
-  }
-  intros x y [Hx | Hy].
-  - destruct x,y.
-    + inversion Hx.
-      apply Nat.pow_nonzero in H0; [destruct H0 | lia].
-    + inversion Hx.
-      apply Nat.pow_nonzero in H0; [destruct H0 | lia].
-    + rewrite (GeqToEqb (S x) (2^m)%nat (2^m-1)%nat); easy.
-    + rewrite (GeqToEqb (S x) (2^m)%nat (2^m-1)%nat); easy.
-  - destruct x,y.
-    + inversion Hy.
-      apply Nat.pow_nonzero in H0; [destruct H0 | lia].
-    + rewrite (GeqToEqb (S y) (2^n)%nat (2^n-1)%nat); [ rewrite andb_false_r; easy | easy | easy].
-    + inversion Hy.
-      apply Nat.pow_nonzero in H0; [destruct H0 | lia].
-    + rewrite (GeqToEqb (S y) (2^n)%nat (2^n-1)%nat); [ rewrite andb_false_r; easy | easy | easy].
-Qed.
-
-Global Hint Resolve WF_Z_semantics : wf_db.
-
-Definition X_semantics (n m : nat) (α : R) : Matrix (2 ^ m) (2 ^ n) :=
-  (m ⨂ hadamard) × (Z_semantics n m α) × (n ⨂ hadamard).
-
-Lemma X_semantics_transpose (n m : nat) (α : R) : (X_semantics n m α) ⊤ = X_semantics m n α.
-Proof.
-  unfold X_semantics.
-  Msimpl.
-  rewrite 2 Mmult_transpose.
-  rewrite 2 kron_n_transpose.
-  Msimpl.
-  restore_dims.
-  rewrite hadamard_st.
-  rewrite <- Mmult_assoc.
-  rewrite Z_semantics_transpose.
-  reflexivity.
-Qed.
-
-Lemma X_semantics_adj (n m : nat) (α : R) : (X_semantics n m α)† = X_semantics m n (- α).
-Proof.
-  unfold X_semantics.
-  rewrite 2 Mmult_adjoint.
-  rewrite <- Mmult_assoc.
-  rewrite Z_semantics_adj.
-  rewrite 2 kron_n_adjoint; try auto with wf_db.
-  rewrite hadamard_sa.
-  reflexivity.
-Qed.
-
-Lemma WF_X_semantics {n m : nat} {α : R} : WF_Matrix (X_semantics n m α).
-Proof.
-  unfold X_semantics.
-  auto with wf_db.
-Qed.
-
-Global Hint Resolve WF_X_semantics : wf_db.
-
-(*
-Lemma WF_Spider_semantics : forall n m bra0 bra1 ket0 ket1 α, 
-                                WF_Matrix bra0 -> WF_Matrix bra1 -> WF_Matrix ket0 -> WF_Matrix ket1 -> 
-                                WF_Matrix (@Spider_semantics bra0 bra1 ket0 ket1 α n m).
-Proof.
-  intros.
-  unfold Spider_semantics.
-  apply WF_plus; restore_dims; try apply WF_scale; apply WF_bra_ket_MN; assumption.
-Qed.
-
-Global Hint Resolve WF_Spider_semantics WF_bra_ket_MN : wf_db.
- *)
-Fixpoint ZX_semantics {nIn nOut} (zx : ZX nIn nOut) : 
-  Matrix (2 ^ nOut) (2 ^nIn) := 
+Fixpoint ZX_semantics {n m} (zx : ZX n m) : 
+  Matrix (2 ^ m) (2 ^n) := 
   match zx with
   | ⦰ => I 1
-  | X_Spider _ _ α => X_semantics nIn nOut α
-  | Z_Spider _ _ α => Z_semantics nIn nOut α
+  | X _ _ α => X_semantics n m α
+  | Z _ _ α => Z_semantics n m α
   | ⊃ => list2D_to_matrix [[C1;C0;C0;C1]]
   | ⊂ => list2D_to_matrix [[C1];[C0];[C0];[C1]]  
   | ⨉ => swap
-  | zx0 ↕ zx1 => (ZX_semantics zx0) ⊗ (ZX_semantics zx1)
+  | — => I 2
+  | □ => hadamard
+  | zx0 ↕ zx1 => (ZX_semantics zx0) ⊗ (ZX_semantics zx1) 
   | zx0 ⟷ zx1 => (ZX_semantics zx1) × (ZX_semantics zx0)
   end.
 
-Lemma ZX_X_is_X_semantics : forall nIn nOut α, (ZX_semantics (X_Spider nIn nOut α) = X_semantics nIn nOut α).
-Proof. easy. Qed.
-
-Lemma ZX_Z_is_Z_semantics : forall nIn nOut α, (ZX_semantics (Z_Spider nIn nOut α) = Z_semantics nIn nOut α).
-Proof. easy. Qed.
-
-Ltac unfold_spider := unfold X_semantics, Z_semantics.
-
-Ltac ZXunfold := simpl; Msimpl; unfold_spider; restore_dims.
-
-Theorem WF_ZX : forall nIn nOut (zx : ZX nIn nOut), WF_Matrix (ZX_semantics zx).
-Proof.
-  intros.
-  induction zx; try (simpl; auto 10 with wf_db);
-  try (simpl; auto 10 with wf_db);
-    apply WF_list2D_to_matrix;
-    try easy; (* case list of length 4 *)
-    try intros; simpl in H; repeat destruct H; try discriminate; try (subst; easy). (* Case of 4 lists length 1 *)
-Qed.
-
-Global Hint Resolve WF_ZX : wf_db.
-
-Definition bra_ket_MN (bra: Matrix 1 2) (ket : Vector 2) {n m} : Matrix (2 ^ m) (2 ^ n) := 
-  (m ⨂ ket) × (n ⨂ bra).
-Transparent bra_ket_MN. 
-
-Lemma WF_bra_ket_MN : forall n m bra ket, WF_Matrix bra -> WF_Matrix ket -> WF_Matrix (@bra_ket_MN bra ket n m).
-Proof.
-  intros.
-  unfold bra_ket_MN.
-  apply WF_mult; restore_dims; apply WF_kron_n; assumption.
-Qed.
-
-Definition Dirac_spider_semantics (bra0 bra1 : Matrix 1 2) (ket0 ket1 : Vector 2) (α : R) {n m : nat} : Matrix (2 ^ m) (2 ^ n) :=
-  (bra_ket_MN bra0 ket0) .+ (Cexp α) .* (bra_ket_MN bra1 ket1). 
-Local Transparent Dirac_spider_semantics.
-
-Lemma WF_Dirac_Spider_semantics : forall n m bra0 bra1 ket0 ket1 α, 
-                                WF_Matrix bra0 -> WF_Matrix bra1 -> WF_Matrix ket0 -> WF_Matrix ket1 -> 
-                                WF_Matrix (@Dirac_spider_semantics bra0 bra1 ket0 ket1 α n m).
-Proof.
-  intros.
-  unfold Dirac_spider_semantics.
-  apply WF_plus; restore_dims; try apply WF_scale; apply WF_bra_ket_MN; assumption.
-Qed.
-
-Global Hint Resolve WF_Dirac_Spider_semantics WF_bra_ket_MN : wf_db.
-
-Fixpoint ZX_Dirac_semantics {nIn nOut} (zx : ZX nIn nOut) : 
-  Matrix (2 ^ nOut) (2 ^nIn) := 
+Fixpoint ZX_dirac_sem {n m} (zx : ZX n m) : 
+  Matrix (2 ^ m) (2 ^n) := 
   match zx with
   | ⦰ => I 1
-  | X_Spider _ _ α => Dirac_spider_semantics (hadamard × (ket 0))† (hadamard × (ket 1))† (hadamard × (ket 0)) (hadamard × (ket 1)) α
-  | Z_Spider _ _ α => Dirac_spider_semantics (bra 0) (bra 1) (ket 0) (ket 1) α
+  | X _ _ α => X_dirac_semantics n m α
+  | Z _ _ α => Z_dirac_semantics n m α
   | ⊃ => list2D_to_matrix [[C1;C0;C0;C1]]
   | ⊂ => list2D_to_matrix [[C1];[C0];[C0];[C1]]  
   | ⨉ => swap
-  | zx0 ↕ zx1 => (ZX_Dirac_semantics zx0) ⊗ (ZX_Dirac_semantics zx1)
-  | zx0 ⟷ zx1 => (ZX_Dirac_semantics zx1) × (ZX_Dirac_semantics zx0)
+  | — => I 2
+  | □ => hadamard
+  | zx0 ↕ zx1 => (ZX_dirac_sem zx0) ⊗ (ZX_dirac_sem zx1)
+  | zx0 ⟷ zx1 => (ZX_dirac_sem zx1) × (ZX_dirac_sem zx0)
   end.
 
-
-Ltac unfold_dirac_spider := simpl; unfold Dirac_spider_semantics, bra_ket_MN; try (simpl; Msimpl).
-
-Ltac ZXDiracunfold := simpl; Msimpl; unfold_spider; restore_dims.
-
-Theorem WF_ZX_Dirac : forall nIn nOut (zx : ZX nIn nOut), WF_Matrix (ZX_Dirac_semantics zx).
+Lemma ZX_semantic_equiv : forall n m (zx : ZX n m),
+  ZX_semantics zx = ZX_dirac_sem zx.
 Proof.
   intros.
-  induction zx; try (simpl; auto 10 with wf_db);
-  try (simpl; auto 10 with wf_db);
+  induction zx; try lma; simpl.
+  rewrite X_semantics_equiv; reflexivity.
+  rewrite Z_semantics_equiv; reflexivity.
+  all: rewrite IHzx1, IHzx2; reflexivity.
+Qed.
+
+Theorem WF_ZX : forall nIn nOut (zx : ZX nIn nOut), WF_Matrix (ZX_semantics zx).
+Proof.
+intros.
+  induction zx; try (simpl; auto 10 with wf_db).
+  1,2: try (simpl; auto 10 with wf_db);
     apply WF_list2D_to_matrix;
     try easy; (* case list of length 4 *)
     try intros; simpl in H; repeat destruct H; try discriminate; try (subst; easy). (* Case of 4 lists length 1 *)
 Qed.
 
-Lemma ZX_Dirac_spider_X_H_Z : forall nIn nOut α, ZX_Dirac_semantics (X_Spider nIn nOut α) = nOut ⨂ hadamard × ZX_Dirac_semantics (Z_Spider nIn nOut α) × (nIn ⨂ hadamard).
-Proof.
-  intros.
-  unfold_dirac_spider.
-  unfold_dirac_spider.
-  repeat rewrite <- kron_n_mult.
-  rewrite Mmult_plus_distr_l.
-  rewrite Mmult_plus_distr_r.
-  apply Mplus_simplify.
-  - repeat rewrite Mmult_assoc. 
-    rewrite hadamard_sa.
-    rewrite ket2bra.
-    reflexivity.
-  - autorewrite with scalar_move_db.
-    apply Mscale_simplify; try reflexivity.
-    rewrite hadamard_sa.
-    rewrite ket2bra.
-    repeat rewrite Mmult_assoc.
-    reflexivity.
-Qed.
-  
-Global Hint Resolve WF_ZX_Dirac : wf_db.
+#[export] Hint Resolve WF_ZX : wf_db.
 
-Definition braket_0_intermediate (n m : nat) : Matrix (2^m) (2^n) :=
-  fun x y => match x, y with
-             | 0, 0 => C1
-             | _, _ => C0
-             end.
-
-Definition braket_1_intermediate (n m : nat) : Matrix (2^m) (2^n) :=
-  fun x y => if (x =? 2^m - 1) && (y =? 2^n - 1) then C1 else C0.
-
-Lemma Z_semantics_split_plus : forall (n m : nat) (α : R), Z_semantics n m α = (braket_0_intermediate n m) .+ Cexp α .* (braket_1_intermediate n m).
-Proof.
-  assert (contra : forall a, (2^S a - 1 <> 0)%nat).
-  { intros; simpl. 
-    destruct (2^a)%nat eqn:Ea. 
-    - apply Nat.pow_nonzero in Ea; [destruct Ea | easy].
-    - simpl; rewrite <- plus_n_Sm; easy.
-  } 
-  intros.
-  unfold braket_0_intermediate; unfold braket_1_intermediate.
-  unfold Z_semantics.
-  unfold Mplus, scale.
-  prep_matrix_equality.
-  destruct x, y; simpl.
-  - destruct (2^n-1)%nat eqn:En, (2^m-1)%nat eqn:Em.
-    + destruct n, m; [lca | destruct (contra m Em) | | ]; destruct (contra n En).
-    + destruct n, m; [discriminate | | | ]; lca.
-    + destruct n, m; [discriminate | | | ]; lca.
-    + destruct n, m; [discriminate | discriminate | | ]; lca.
-  - destruct (2^n-1)%nat eqn:En, (2^m-1)%nat eqn:Em.
-    + destruct n,m; [lca | destruct (contra m Em) | | ]; destruct (contra n En).
-    + destruct n, m; [discriminate | | | ]; lca.
-    + destruct n, m; [discriminate | discriminate | |]; destruct (y =? n0); lca.
-    + destruct n, m; [discriminate | | | lca]; destruct (y =? n0); lca.
-  - destruct (2^n-1)%nat eqn:En, (2^m-1)%nat eqn:Em; [lca | | lca | ]; destruct (_ =? _); lca.
-  - destruct (2^n-1)%nat eqn:En, (2^m-1)%nat eqn:Em; [lca | | lca | ]; repeat destruct (_ =? _); lca.
-Qed.
-
-Lemma big_bra_0_0_0 : forall n, (n ⨂ (bra 0)) 0 0 = C1.
-Proof.
-  intros.
-  induction n; [reflexivity | ].
-  rewrite kron_n_assoc; [ | auto with wf_db].
-  unfold kron.
-  rewrite 2 Nat.div_0_l; try apply Nat.pow_nonzero; try easy.
-  rewrite 2 Nat.mod_0_l; try apply Nat.pow_nonzero; try easy.
-  rewrite IHn.
-  rewrite Cmult_1_r.
-  unfold bra.
-  unfold adjoint.
-  simpl.
-  lca.
-Qed.
-
-Lemma big_bra_S_r : forall n i j, ((S n) ⨂ bra 0) i (S j) = C0.
-Proof.
-  induction n.
-  - simpl; rewrite kron_1_l; [ | auto with wf_db ].
-    intros; unfold bra; simpl; unfold adjoint; unfold qubit0.
-    destruct i,j; lca.
-  - intros.
-    rewrite kron_n_assoc; [| auto with wf_db].
-    unfold kron.
-    destruct (S j mod 2 ^S n) eqn:En.
-    + destruct (Nat.mod_divides (S j) (2 ^ S n)); [apply Nat.pow_nonzero; auto |]. 
-      destruct (H En).
-      rewrite H1.
-      replace (2 ^ S n * x / 2 ^ S n)%nat with x.
-      * unfold bra; simpl.
-        unfold adjoint.
-        simpl.
-        destruct x.
-        -- rewrite mult_0_r in H1.
-           discriminate H1.
-        -- destruct (i / (1 ^ n + 0))%nat. 
-           ++ simpl.
-              destruct x; lca.
-           ++ simpl.
-              destruct x; lca.
-      * rewrite mult_comm.
-        rewrite Nat.divide_div_mul_exact.
-        -- rewrite Nat.div_same; [lia | ].
-           apply Nat.pow_nonzero; easy.
-        -- apply Nat.pow_nonzero; easy.
-        -- apply Nat.divide_refl.
-    + rewrite IHn.
-      lca.
-Qed.
-
-Lemma big_bra_S_l : forall n i j, (n ⨂ bra 0) (S i) j = C0.
-Proof.
-  intros.
-  assert (WF : WF_Matrix (n ⨂ bra 0)).
-  { auto with wf_db. }
-  apply WF.
-  left.
-  rewrite Nat.pow_1_l.
-  induction i; auto.
-Qed.
-
-Lemma big_ket_0_0_0 : forall n, (n ⨂ (ket 0)) 0 0 = C1.
-Proof.
-  intros.
-  induction n; [reflexivity | ].
-  rewrite kron_n_assoc; [ | auto with wf_db].
-  unfold kron.
-  rewrite 2 Nat.div_0_l; try apply Nat.pow_nonzero; try easy.
-  rewrite 2 Nat.mod_0_l; try apply Nat.pow_nonzero; try easy.
-  rewrite IHn.
-  rewrite Cmult_1_r.
-  reflexivity.
-Qed.
-
-Lemma big_ket_S_r : forall n i j, (n ⨂ ket 0) i (S j) = C0.
-Proof.
-  intros.
-  assert (WF : WF_Matrix (n ⨂ ket 0)).
-  { auto with wf_db. }
-  apply WF.
-  right.
-  rewrite Nat.pow_1_l.
-  induction j; auto.
-Qed.
-
-Lemma big_ket_S_l : forall n i j, (S n ⨂ ket 0) (S i) j = C0.
-Proof.
-  induction n.
-  - intros. simpl.
-    rewrite kron_1_l; [ | auto with wf_db ].
-    unfold ket.
-    unfold qubit0; simpl.
-    destruct i, j;lca.
-  - intros.
-    rewrite kron_n_assoc; [ | auto with wf_db ].
-    unfold kron.
-    rewrite Nat.pow_1_l.
-    rewrite Nat.mod_1_r.
-    rewrite Nat.div_1_r.
-    destruct (S i mod 2 ^ S n) eqn:En.
-    + destruct (Nat.mod_divides (S i) (2^S n)); [apply Nat.pow_nonzero; auto |].
-      destruct H; [assumption |].
-      rewrite H.
-      rewrite mult_comm.
-      rewrite Nat.divide_div_mul_exact; [ | apply Nat.pow_nonzero; auto | apply Nat.divide_refl ].
-      rewrite Nat.div_same; [ | apply Nat.pow_nonzero; auto].
-      rewrite Nat.mul_1_r.
-      destruct x; [rewrite mult_0_r in H; discriminate H |].
-      unfold ket; simpl.
-      destruct x, j; lca.
-    + rewrite IHn.
-      lca.
-Qed.
-
-Lemma braket_sem_0_intermediate : forall (n m : nat), (n ⨂ ket 0) × (m ⨂ bra 0) = braket_0_intermediate m n.
-Proof.
-  intros.
-  destruct n,m; prep_matrix_equality.
-  - destruct x,y; lca.
-  - unfold Mmult; simpl.
-    destruct x,y; replace (m ⨂ bra 0 ⊗ bra 0) with ((S m) ⨂ bra 0) by reflexivity.
-    + rewrite big_bra_0_0_0.
-      lca.
-    + rewrite big_bra_S_r.
-      lca.
-    + rewrite big_bra_0_0_0.
-      lca.
-    + rewrite big_bra_S_r.
-      lca.
-  - unfold Mmult; rewrite Nat.pow_1_l; simpl.
-    destruct x,y; replace (n ⨂ ket 0 ⊗ ket 0) with ((S n) ⨂ ket 0) by reflexivity.
-    + rewrite big_ket_0_0_0.
-      lca.
-    + rewrite big_ket_0_0_0.
-      lca.
-    + rewrite big_ket_S_l.
-      lca.
-    + rewrite big_ket_S_l.
-      lca.
-  - unfold Mmult; rewrite Nat.pow_1_l; simpl; rewrite Cplus_0_l.
-    replace (n ⨂ ket 0 ⊗ ket 0) with ((S n) ⨂ ket 0) by reflexivity;
-    replace (m ⨂ bra 0 ⊗ bra 0) with ((S m) ⨂ bra 0) by reflexivity.
-    destruct x,y.
-    + rewrite big_ket_0_0_0; rewrite big_bra_0_0_0.
-      lca.
-    + rewrite big_bra_S_r.
-      lca.
-    + rewrite big_ket_S_l.
-      lca.
-    + rewrite big_ket_S_l.
-      lca.
-Qed.
-
-Lemma big_ket_1_max_0 : forall n, (n ⨂ (ket 1)) (2 ^ n - 1)%nat 0 = C1.
-Proof.
-  induction n.
-  - lca.
-  - rewrite kron_n_assoc; [| auto with wf_db].
-    unfold kron.
-    simpl.
-    rewrite <- Nat.add_sub_assoc.
-    + replace (0 / 1 ^ n)%nat with 0%nat by (rewrite Nat.pow_1_l; rewrite Nat.div_1_r; reflexivity).
-      replace (0 mod 1^n) with 0 by (rewrite Nat.pow_1_l; reflexivity).
-      replace ((2 ^ n + (2 ^ n + 0 - 1)) / 2 ^ n)%nat with 1%nat.
-      * replace ((2 ^ n + (2 ^ n + 0 - 1)) mod 2 ^ n)%nat with (2^n-1)%nat.
-        -- rewrite IHn; lca.
-        -- rewrite Nat.add_mod; [| apply Nat.pow_nonzero; auto].
-           ++ rewrite plus_0_r.
-              rewrite Nat.mod_same; [| apply Nat.pow_nonzero; auto].
-              rewrite plus_0_l.
-              rewrite Nat.mod_mod; [| apply Nat.pow_nonzero; auto].
-              destruct n.
-              ** reflexivity.
-              ** rewrite Nat.mod_small; [reflexivity|].
-                 destruct (2 ^ S n)%nat eqn:E.
-                 --- destruct (Nat.pow_nonzero 2 (S n)); [auto |apply E].
-                 --- simpl.
-                     rewrite Nat.sub_0_r.
-                     constructor.
-      * rewrite plus_0_r.
-        replace ((2 ^ n + (2 ^ n - 1)) / 2 ^ n)%nat with (((1 * 2 ^ n) + (2 ^ n - 1)) / 2 ^ n)%nat.
-        -- rewrite Nat.div_add_l; [| apply Nat.pow_nonzero; auto].
-           rewrite Nat.div_small; [reflexivity|].
-           destruct (2^n)%nat eqn:E.
-           ++ destruct (Nat.pow_nonzero 2 n); [auto | apply E].
-           ++ simpl; rewrite Nat.sub_0_r.
-              auto.
-        -- rewrite mult_1_l.
-           reflexivity.
-    + rewrite plus_0_r.
-      rewrite <- (Nat.pow_1_l n).
-      replace (S (1 ^ n)) with 2.
-      * apply Nat.pow_le_mono_l.
-        auto.
-      * rewrite Nat.pow_1_l; reflexivity.
-Qed.
-
-Lemma big_bra_1_0_max : forall n, (n ⨂ (bra 1)) 0 (2 ^ n - 1)%nat = C1.
-Proof.
-  induction n.
-  - lca.
-  - rewrite kron_n_assoc; [| auto with wf_db].
-    unfold kron.
-    simpl.
-    rewrite <- Nat.add_sub_assoc.
-    + replace (0 / 1 ^ n)%nat with 0%nat by (rewrite Nat.pow_1_l; rewrite Nat.div_1_r; reflexivity).
-      replace (0 mod 1^n) with 0 by (rewrite Nat.pow_1_l; reflexivity).
-      replace ((2 ^ n + (2 ^ n + 0 - 1)) / 2 ^ n)%nat with 1%nat.
-      * replace ((2 ^ n + (2 ^ n + 0 - 1)) mod 2 ^ n)%nat with (2^n-1)%nat.
-        -- rewrite IHn; lca.
-        -- rewrite Nat.add_mod; [| apply Nat.pow_nonzero; auto].
-           ++ rewrite plus_0_r.
-              rewrite Nat.mod_same; [| apply Nat.pow_nonzero; auto].
-              rewrite plus_0_l.
-              rewrite Nat.mod_mod; [| apply Nat.pow_nonzero; auto].
-              destruct n.
-              ** reflexivity.
-              ** rewrite Nat.mod_small; [reflexivity|].
-                 destruct (2 ^ S n)%nat eqn:E.
-                 --- destruct (Nat.pow_nonzero 2 (S n)); [auto |apply E].
-                 --- simpl.
-                     rewrite Nat.sub_0_r.
-                     constructor.
-      * rewrite plus_0_r.
-        replace ((2 ^ n + (2 ^ n - 1)) / 2 ^ n)%nat with (((1 * 2 ^ n) + (2 ^ n - 1)) / 2 ^ n)%nat.
-        -- rewrite Nat.div_add_l; [| apply Nat.pow_nonzero; auto].
-           rewrite Nat.div_small; [reflexivity|].
-           destruct (2^n)%nat eqn:E.
-           ++ destruct (Nat.pow_nonzero 2 n); [auto | apply E].
-           ++ simpl; rewrite Nat.sub_0_r.
-              auto.
-        -- rewrite mult_1_l.
-           reflexivity.
-    + rewrite plus_0_r.
-      rewrite <- (Nat.pow_1_l n).
-      replace (S (1 ^ n)) with 2.
-      * apply Nat.pow_le_mono_l.
-        auto.
-      * rewrite Nat.pow_1_l; reflexivity.
-Qed.
-
-Lemma big_ket_1_n_S : forall n i j, (n ⨂ (ket 1)) i (S j) = C0.
-Proof.
-  induction n.
-  - intros.
-    simpl.
-    destruct i.
-    + lca.
-    + unfold I.
-      replace (S i <? 1) with false; [| reflexivity].
-      rewrite andb_false_r.
-      reflexivity.
-  - intros.
-    simpl.
-    unfold kron.
-    rewrite Nat.div_1_r.
-    rewrite IHn.
-    lca.
-Qed.
-
-Definition big_bra_sem (n : nat) : Matrix 1 (2 ^ n) :=
-  fun x y => 
-  if (y =? 2^n-1) && (x =? 0) then C1 else C0.
-
-Lemma big_bra_to_sem : forall n, (n ⨂ (bra 1)) = big_bra_sem n.
-Proof.
-  induction n.
-  - prep_matrix_equality.
-    destruct x,y.
-    + lca.
-    + lca.
-    + lca.
-    + unfold big_bra_sem.
-      rewrite andb_false_r.
-      simpl.
-      unfold I.
-      rewrite andb_false_r.
-      reflexivity.
-  - prep_matrix_equality.
-    simpl.
-    rewrite IHn.
-    unfold kron.
-    destruct (y =? 2^(S n) - 1) eqn:Ex.
-    + unfold big_bra_sem.
-      rewrite Ex.
-      apply Nat.eqb_eq in Ex.
-      rewrite Ex.
-      rewrite Nat.mod_1_r.
-      rewrite Nat.div_1_r.
-      destruct y.
-      * destruct (2^n)%nat eqn:En.
-        -- contradict En.
-           apply Nat.pow_nonzero.
-           easy.
-        -- replace ((2 ^ S n - 1) / 2)%nat with (2^n - 1)%nat.
-           ++ rewrite En.
-              rewrite Nat.eqb_refl.
-              replace ((2 ^ S n - 1) mod 2)%nat with 1%nat.
-              ** destruct x; lca.
-              ** replace (2 ^ S n)%nat with (2^n + 2^n)%nat.
-                 --- destruct (2 ^ n)%nat eqn:E2n.
-                     +++ contradict E2n.
-                         apply Nat.pow_nonzero; easy.
-                     +++ rewrite <- plus_n_Sm.
-                         replace (S (S n1 + n1) - 1)%nat with (S (n1 + n1))%nat by reflexivity.
-                         rewrite (double_mult n1).
-                         rewrite <- (plus_0_l (2*n1)).
-                         replace (S (0 + 2 * n1))%nat with (1 + 2 * n1)%nat by reflexivity.
-                         rewrite Nat.add_mod; [| easy].
-                         rewrite mult_comm.
-                         rewrite Nat.mod_mul; [| easy].
-                         reflexivity.
-                 --- simpl.
-                     rewrite plus_0_r.
-                     lia.
-           ++ replace (2 ^ S n)%nat with (2 * (2 ^ n))%nat.
-              ** destruct (2^n)%nat.
-                 --- reflexivity.
-                 --- contradict Ex.
-                     destruct (2^S n)%nat eqn:Esn.
-                     +++ contradict Esn.
-                         apply Nat.pow_nonzero; easy.
-                     +++ destruct n2.
-                         *** contradict Esn.
-                             simpl.
-                             destruct (2^n)%nat.
-                             ---- easy.
-                             ---- destruct n2.
-                                  ++++ easy.
-                                  ++++ simpl.
-                                       easy.
-                         *** easy.
-              ** reflexivity.
-      * Opaque Nat.div.
-        Opaque Nat.modulo.
-        replace ((2 ^ S n - 1) / 2)%nat with (2^n - 1)%nat.
-        replace ((2 ^ S n - 1) mod 2)%nat with 1%nat.
-        -- rewrite Nat.eqb_refl.
-           destruct x; lca.
-        -- simpl.
-           rewrite plus_0_r.
-           destruct (2 ^ n)%nat eqn:En.
-           ++ contradict En.
-              ** apply Nat.pow_nonzero; easy.
-           ++ simpl.
-              rewrite <- plus_n_Sm.
-              rewrite Nat.sub_0_r.
-              rewrite double_mult.
-              replace (S (2 * n0))%nat with (1 + (2 * n0))%nat by reflexivity.
-              rewrite mult_comm.
-              rewrite Nat.add_mod; [| easy].
-              rewrite Nat.mod_mul; [| easy].
-              reflexivity.
-        -- simpl.
-           rewrite plus_0_r.
-           destruct (2 ^ n)%nat.
-           ++ reflexivity.
-           ++ simpl.
-              rewrite Nat.sub_0_r.
-              rewrite Nat.sub_0_r.
-              rewrite <- plus_n_Sm.
-              rewrite double_mult.
-              replace (S (2 * n0))%nat with ((1 + (2 * n0)))%nat by reflexivity.
-              rewrite plus_comm.
-              rewrite mult_comm.
-              rewrite Nat.div_add_l; [| easy].
-              rewrite plus_comm.
-              reflexivity.
-    + unfold big_bra_sem.
-      rewrite Ex.
-      simpl.
-      rewrite Nat.mod_1_r.
-      Transparent Nat.div.
-      destruct (Nat.divmod y 1 0 1) eqn:Edm.
-      assert (Hy : (y = 2 * (y / 2) + y mod 2)%nat).
-      { apply Nat.div_mod; lia. } (* Nat.div_mod_eq works in 8.14 on *)
-      destruct (y/2 =? 2^n-1) eqn:Ey2.
-      * destruct (y mod 2 =? 1) eqn:Eym.
-        -- apply Nat.eqb_eq in Eym, Ey2.
-           rewrite Ey2, Eym in Hy.
-           replace (2 * (2 ^ n - 1) + 1)%nat with (2 ^ S n - 1)%nat in Hy.
-           ++ rewrite Hy in Ex.
-              rewrite Nat.eqb_refl in Ex.
-              discriminate.
-           ++ simpl.
-              rewrite 2 plus_0_r.
-              rewrite <- plus_assoc.
-              rewrite <- plus_n_Sm.
-              rewrite plus_0_r.
-              destruct (2 ^ n)%nat eqn:En.
-              ** contradict En.
-                 apply Nat.pow_nonzero; easy.
-              ** simpl. lia.
-        -- destruct (y mod 2).
-           ++ lca.
-           ++ destruct n2.
-              ** discriminate.
-              ** lca.
-      * lca.
-Qed.
-
-Definition big_ket_sem (n : nat) : Matrix (2 ^ n) 1 :=
-  fun x y => 
-  if (x =? 2^n-1) && (y =? 0) then C1 else C0.
-
-Lemma big_ket_sem_big_bra_sem_transpose : forall n, big_ket_sem n = (big_bra_sem n) ⊤.
-Proof.
-  intros.
-  solve_matrix.
-Qed.
-
-Lemma big_ket_to_sem : forall n, (n ⨂ (ket 1)) = big_ket_sem n.
-Proof.
-  intros.
-  rewrite <- (transpose_involutive _ _ _).
-  rewrite kron_n_transpose.
-  replace ((ket 1)⊤) with (bra 1).
-  - rewrite big_ket_sem_big_bra_sem_transpose.
-    f_equal.
-    + rewrite Nat.pow_1_l.
-      easy.
-    + apply big_bra_to_sem.
-  - solve_matrix.
-Qed.
-
-Lemma braket_sem_1_intermediate : forall n m : nat, n ⨂ ket 1 × m ⨂ bra 1 = braket_1_intermediate m n.
-Proof.
-  intros.
-  rewrite big_bra_to_sem.
-  rewrite big_ket_to_sem.
-  prep_matrix_equality.
-  unfold braket_1_intermediate, big_ket_sem, big_bra_sem, Mmult.
-  rewrite Nat.pow_1_l; simpl.
-  rewrite Cplus_0_l.
-  destruct (x =? 2^n-1), (y =? 2^m-1); lca.
-Qed.
-
-Lemma ZX_Z_semantics_equiv : forall nIn nOut α, ZX_semantics (Z_Spider nIn nOut α) = ZX_Dirac_semantics (Z_Spider nIn nOut α).
-Proof.
-  assert (contra : forall a, (0 =? 2 ^ S a - 1) = false).
-  { intros.
-    simpl.
-    destruct (2^a)%nat eqn:Ea.
-    - contradict Ea.
-      apply Nat.pow_nonzero; easy.
-    - rewrite plus_0_r.
-      rewrite <- plus_n_Sm. easy.
-  }
-  intros.
-  simpl.
-  unfold_dirac_spider.
-  rewrite (braket_sem_0_intermediate nOut nIn).
-  rewrite (braket_sem_1_intermediate nOut nIn).
-  apply Z_semantics_split_plus.
-Qed.
-
-Lemma ZX_X_semantics_equiv : forall nIn nOut α, ZX_semantics (X_Spider nIn nOut α) = ZX_Dirac_semantics (X_Spider nIn nOut α).
-Proof.
-  intros.
-  simpl.
-  unfold X_semantics.
-  unfold_dirac_spider.
-  repeat rewrite <- kron_n_mult.
-  replace (nOut ⨂ hadamard × nOut ⨂  ket 1 × (nIn ⨂  (ket 1) † × nIn ⨂ (hadamard) †)) 
-    with (nOut  ⨂ hadamard × ((nOut ⨂  ket 1) × (nIn ⨂ (ket 1) †)) × nIn ⨂ (hadamard) †).
-  replace (nOut ⨂ hadamard × nOut ⨂ ∣ 0 ⟩ × (nIn ⨂ (∣ 0 ⟩) † × nIn ⨂ (hadamard) †)) 
-    with (nOut ⨂ hadamard × ((nOut ⨂  ket 0) × (nIn ⨂ (ket 0) †)) × nIn ⨂ (hadamard) †).
-    - rewrite <- Mscale_mult_dist_l.
-      rewrite <- Mscale_mult_dist_r.
-      rewrite <- Mmult_plus_distr_r.
-      rewrite <- Mmult_plus_distr_l.
-      assert (H : forall nIn nOut α, ZX_semantics (Z_Spider nIn nOut α) = ZX_Dirac_semantics (Z_Spider nIn nOut α)).
-      { apply ZX_Z_semantics_equiv. } 
-      simpl in H.
-      unfold Dirac_spider_semantics in H.
-      unfold bra_ket_MN in H.
-      rewrite <- H.
-      rewrite hadamard_sa.
-      reflexivity.
-    - repeat rewrite Mmult_assoc.
-      reflexivity.
-    - repeat rewrite Mmult_assoc.
-      reflexivity.
-Qed.
-
-Transparent Nat.div.
-Transparent Nat.modulo.
-
-Theorem ZX_semantics_equiv (nIn nOut : nat) : forall (zx : ZX nIn nOut),
-  ZX_semantics zx = ZX_Dirac_semantics zx.
-Proof.
-  intros.
-  induction zx; try auto.
-  - apply ZX_X_semantics_equiv.
-  - apply ZX_Z_semantics_equiv.
-  - simpl.
-    rewrite IHzx1, IHzx2.
-    reflexivity.
-  - simpl.
-    rewrite IHzx1, IHzx2.
-    reflexivity.
-Qed.
-
-Definition Wire : ZX 1 1 := Z_Spider _ _ 0.
-
-Notation "—" := Wire. (* \emdash *)
-
-Theorem wire_identity_semantics : ZX_semantics — = I 2.
-Proof.
-  simpl.
-  unfold Z_semantics.
-  unfold I.
-  prep_matrix_equality.
-  rewrite Cexp_0.
-  simpl.
-  destruct x; destruct y; try reflexivity.
-  - simpl.
-    destruct x; reflexivity.
-  - simpl.
-    destruct x; destruct y; try reflexivity.
-    + simpl.
-      unfold Nat.ltb.
-      unfold Nat.leb.
-      rewrite andb_false_r.
-      reflexivity.
-Qed.
-
-Global Opaque Wire.
-
-Global Hint Resolve wire_identity_semantics : zx_sem_db.
+(* Parametrized diagrams *)
 
 Reserved Notation "n ⇑ zx" (at level 40). (* \Uparrow - maybe change to ⇕ (\Updownarrow) *)
 Fixpoint nStack {nIn nOut} n (zx : ZX nIn nOut) : ZX (n * nIn) (n * nOut) :=
@@ -880,119 +120,146 @@ Proof.
 Qed.
 
 Definition nWire := fun n => n ↑ Wire.
+Definition nBox := fun n => n ↑ Box.
 
-Global Opaque nWire.
+Lemma nWire_semantics {n} : ZX_semantics (nWire n) = I (2^n).
+Proof.
+  induction n; auto.
+  simpl.
+  unfold nWire in IHn.
+  rewrite IHn.
+  rewrite id_kron.
+  auto.
+Qed.
 
-(* Definitions for transposes of ZX diagrams and a proof that its what we expect *)
-Reserved Notation "zx ⊺" (at level 10). (* \intercal *)
-Fixpoint Transpose {nIn nOut} (zx : ZX nIn nOut) : ZX nOut nIn :=
+Lemma nBox_semantics {n} : ZX_semantics (nBox n) = n ⨂ hadamard.
+Proof.
+  induction n; auto.
+  simpl.
+  unfold nBox in IHn.
+  rewrite IHn.
+  rewrite <- kron_n_assoc by auto with wf_db.
+  auto.
+Qed.
+
+#[export] Hint Rewrite @nWire_semantics @nBox_semantics : zx_sem_db.
+
+Global Opaque nWire nBox.
+
+(** Global operations on ZX diagrams *)
+
+(* Transpose of a diagram *)
+
+Reserved Notation "zx ⊤" (at level 0). (* \top *)
+Fixpoint transpose {nIn nOut} (zx : ZX nIn nOut) : ZX nOut nIn :=
   match zx with
   | ⦰ => ⦰
-  | Z_Spider mIn mOut α => Z_Spider mOut mIn α
-  | X_Spider mIn mOut α => X_Spider mOut mIn α
-  | zx1 ⟷ zx2 => (zx2 ⊺) ⟷ (zx1 ⊺)
-  | zx1 ↕ zx2 => (zx1 ⊺) ↕ (zx2 ⊺)
+  | Z mIn mOut α => Z mOut mIn α
+  | X mIn mOut α => X mOut mIn α
+  | zx1 ⟷ zx2 => (zx2 ⊤) ⟷ (zx1 ⊤)
+  | zx1 ↕ zx2 => (zx1 ⊤) ↕ (zx2 ⊤)
   | ⊂ => ⊃
   | ⊃ => ⊂
-  | ⨉ => ⨉
+  | other => other
   end
-  where "zx ⊺" := (Transpose zx).
+  where "zx ⊤" := (transpose zx) : ZX_scope.
 
 Lemma transpose_involutive_eq : forall {nIn nOut} (zx : ZX nIn nOut),
-  zx = (zx ⊺)⊺.
+  zx = (zx ⊤)⊤.
 Proof.
   intros; induction zx; try auto.
   all: simpl; rewrite <- IHzx1, <- IHzx2; auto.
 Qed.
 
+(* Negating the angles of a diagram, complex conjugate *)
 
-Fixpoint Invert_angles {nIn nOut} (zx : ZX nIn nOut) : ZX nIn nOut :=
+Reserved Notation "zx ^*" (at level 10).
+Fixpoint conjugate {n m} (zx : ZX n m) : ZX n m :=
   match zx with
-  | Z_Spider mIn mOut α => Z_Spider mIn mOut (-α)
-  | X_Spider mIn mOut α => X_Spider mIn mOut (-α)
-  | zx1 ⟷ zx2 => (Invert_angles zx1) ⟷ (Invert_angles zx2)
-  | zx1 ↕ zx2 => (Invert_angles zx1) ↕ (Invert_angles zx2)
+  | Z n m α => Z n m (-α)
+  | X n m α => X n m (-α)
+  | zx1 ⟷ zx2 => zx1^* ⟷ zx2^*
+  | zx1 ↕ zx2 => zx1^* ↕ zx2^*
   | other => other
-  end.
+  end
+  where "zx ^*" := (conjugate zx) : ZX_scope.
 
-Definition Adjoint {nIn nOut} (zx : ZX nIn nOut) : ZX nOut nIn := Invert_angles (zx ⊺).
-Notation "zx ‡" := (Adjoint zx) (at level 10). (* \ddagger *)
+Definition adjoint {n m} (zx : ZX n m) : ZX m n :=
+  (zx^*)⊤.
+Notation "zx †" := (adjoint zx) (at level 0) : ZX_scope.
 
-
-Lemma ZX_semantics_Transpose_comm {nIn nOut} : forall (zx : ZX nIn nOut),
-  ZX_semantics (zx ⊺) = (ZX_semantics zx) ⊤.
+Lemma ZX_semantics_transpose_comm {nIn nOut} : forall (zx : ZX nIn nOut),
+  ZX_semantics (zx ⊤) = ((ZX_semantics zx) ⊤)%M.
 Proof.
-  assert (Mmult_trans_dep : forall n m o p (A : Matrix n m) (B : Matrix o p), m = o -> (A × B) ⊤ = B ⊤ × A ⊤).
+  assert (Mmult_trans_dep : forall n m o p (A : Matrix n m) (B : Matrix o p), m = o -> ((A × B) ⊤ = B ⊤ × A ⊤)%M).
     {
       intros; rewrite Mmult_transpose; rewrite H in *; reflexivity.      
     }
   induction zx.
-  - Msimpl.
-    reflexivity.
-  - simpl.
-    rewrite X_semantics_transpose.
-    reflexivity.
-  - simpl.
-    rewrite Z_semantics_transpose.
-    reflexivity.
+  - Msimpl; reflexivity.
   - simpl; solve_matrix.
   - simpl; solve_matrix.
-  - simpl; solve_matrix.
+  - simpl; lma.
+  - simpl; rewrite id_transpose_eq; reflexivity.
+  - simpl; rewrite hadamard_st; reflexivity.
+  - simpl; rewrite X_semantics_transpose; reflexivity.
+  - simpl; rewrite Z_semantics_transpose; reflexivity.
   - simpl; rewrite IHzx1, IHzx2; rewrite <- kron_transpose; reflexivity.
   - simpl; rewrite IHzx1, IHzx2; rewrite <- Mmult_transpose; reflexivity.
 Qed.
 
-Lemma ZX_semantics_Adjoint_comm {nIn nOut} : forall (zx : ZX nIn nOut),
-  ZX_semantics (zx ‡) = (ZX_semantics zx) †.
+
+Lemma ZX_semantics_adjoint_comm {nIn nOut} : forall (zx : ZX nIn nOut),
+  ZX_semantics (zx †) = (ZX_semantics zx) †%M.
 Proof.
   intros.
   induction zx.
-  1, 4, 5, 6: ZXunfold; solve_matrix. (* Cap, Cup, Swap *)
-  3, 4: simpl; unfold Adjoint in IHzx1; unfold Adjoint in IHzx2; rewrite IHzx1, IHzx2;
-        try rewrite <- kron_adjoint; try rewrite <- Mmult_adjoint;
-        reflexivity. (* Compose, Stack *)
-  - simpl.
-    rewrite X_semantics_adj.
-    reflexivity.
-  - simpl.
-    rewrite Z_semantics_adj.
-    reflexivity.
+  - simpl; Msimpl; reflexivity.
+  - simpl; solve_matrix.
+  - simpl; solve_matrix.
+  - simpl; lma.
+  - simpl; Msimpl; reflexivity.
+  - simpl; lma.
+  - simpl; rewrite X_semantics_adj; reflexivity.
+  - simpl; rewrite Z_semantics_adj; reflexivity.
+  - simpl; fold (zx1†); fold (zx2†); rewrite IHzx1, IHzx2; rewrite <- kron_adjoint; reflexivity.
+  - simpl; fold (zx1†); fold(zx2†); rewrite IHzx1, IHzx2; rewrite Mmult_adjoint; reflexivity.
 Qed.
+
+Opaque adjoint.
 
 Reserved Notation "⊙ zx" (at level 10). (* \odot *) 
 Fixpoint ColorSwap {nIn nOut} (zx : ZX nIn nOut) : ZX nIn nOut := 
   match zx with
-  | X_Spider n m α  => Z_Spider n m α
-  | Z_Spider n m α  => X_Spider n m α
+  | X n m α  => Z n m α
+  | Z n m α  => X n m α
   | zx1 ↕ zx2   => (⊙ zx1) ↕ (⊙ zx2)
   | zx1 ⟷ zx2 => (⊙ zx1) ⟷ (⊙ zx2)
   | otherwise => otherwise
   end
-  where "⊙ zx" := (ColorSwap zx).
-
-Local Open Scope C_scope.
+  where "⊙ zx" := (ColorSwap zx) : ZX_scope.
 
 Lemma ZX_semantics_Colorswap_comm {nIn nOut} : forall (zx : ZX nIn nOut),
   ZX_semantics (⊙ zx) = nOut ⨂ hadamard × (ZX_semantics zx) × nIn ⨂ hadamard.
 Proof.
   induction zx.
-  - ZXunfold; reflexivity.
+  - simpl; Msimpl; reflexivity.
+  - solve_matrix.
+  - solve_matrix.
   - simpl.
-    unfold X_semantics.
+    Msimpl.
+    solve_matrix.
+  - simpl; Msimpl; restore_dims; rewrite MmultHH; reflexivity.
+  - simpl; Msimpl; restore_dims; rewrite MmultHH; Msimpl; reflexivity.
+  - simpl. unfold X_semantics.
     rewrite <- 2 Mmult_assoc.
     rewrite kron_n_mult.
     rewrite 2 Mmult_assoc.
     rewrite kron_n_mult.
     rewrite MmultHH.
     rewrite 2 kron_n_I.
-    rewrite Mmult_1_r; try auto with wf_db.
-    rewrite Mmult_1_l; try auto with wf_db.
+    Msimpl; reflexivity.
   - reflexivity.
-  - solve_matrix.
-  - solve_matrix.
-  - simpl.
-    Msimpl.
-    solve_matrix.
   - simpl.
     rewrite IHzx1, IHzx2.
     rewrite 2 kron_n_m_split; try auto with wf_db.
@@ -1002,11 +269,11 @@ Proof.
   - simpl.
     rewrite IHzx1, IHzx2.
     rewrite Mmult_assoc.
-    rewrite <- 2 Mmult_assoc with (nMid ⨂ hadamard) _ _.
+    rewrite <- 2 Mmult_assoc with (m ⨂ hadamard) _ _.
     rewrite kron_n_mult.
     rewrite MmultHH.
     rewrite kron_n_I.
-    rewrite Mmult_1_l; [| apply WF_ZX].
+    Msimpl.
     repeat rewrite Mmult_assoc.
     reflexivity.
 Qed.
