SemanticCore.v
@@ -1,0 +1,681 @@
+(** Contains the definitions for Z and X spider semantics, their equivalence, and well
+    formedness *)
+
+Require Export externals.QuantumLib.Quantum.
+Require Export externals.QuantumLib.Proportional.
+Require Export externals.QuantumLib.VectorStates.
+
+
+(* Sparse Matrix Definition *)
+
+Definition Z_semantics (n m : nat) (α : R) : Matrix (2 ^ m) (2 ^ n) :=
+  fun x y =>
+  match x, y with
+  | 0, 0 => match n, m with
+                  | 0, 0 => C1 + Cexp α
+                  | _, _  => C1
+                  end
+  | _, _ => if ((x =? 2^m-1) && (y =? 2^n-1)) then Cexp α else C0
+  end.
+
+Definition X_semantics (n m : nat) (α : R) : Matrix (2 ^ m) (2 ^ n) :=
+  (m ⨂ hadamard) × (Z_semantics n m α) × (n ⨂ hadamard).
+
+
+(* Transpose and Adjoint lemmas *)
+
+Lemma Z_semantics_transpose (n m : nat) (α : R) : (Z_semantics n m α) ⊤ = Z_semantics m n α.
+Proof.
+  unfold Z_semantics.
+  unfold transpose.
+  prep_matrix_equality.
+  destruct x, y.
+  1: destruct n, m; reflexivity.
+  all: rewrite andb_comm; reflexivity.
+Qed.
+
+Lemma Z_semantics_adj (n m : nat) (α : R) : (Z_semantics n m α) † = Z_semantics m n (- α).
+Proof.
+  unfold adjoint.
+  unfold Z_semantics.
+  prep_matrix_equality.
+  destruct x,y. 
+  1: destruct n,m; try lca;
+    rewrite Cconj_plus_distr;
+    rewrite Cexp_conj_neg;
+    lca.
+  all: rewrite andb_comm;
+       rewrite (if_dist _ _ _ (Cconj));
+       rewrite Cexp_conj_neg;
+       rewrite Cconj_0;
+       reflexivity.
+Qed.
+
+Lemma X_semantics_transpose (n m : nat) (α : R) : (X_semantics n m α) ⊤ = X_semantics m n α.
+Proof.
+  unfold X_semantics.
+  rewrite 2 Mmult_transpose.
+  rewrite 2 kron_n_transpose.
+  rewrite hadamard_st.
+  rewrite Mmult_assoc.
+  rewrite Z_semantics_transpose.
+  reflexivity.
+Qed.
+
+Lemma X_semantics_adj (n m : nat) (α : R) : (X_semantics n m α)† = X_semantics m n (- α).
+Proof.
+  unfold X_semantics.
+  distribute_adjoint.
+  rewrite Z_semantics_adj.
+  rewrite 2 kron_n_adjoint; try auto with wf_db.
+  rewrite hadamard_sa.
+  rewrite Mmult_assoc.
+  reflexivity.
+Qed.
+
+
+(* Dirac Notation *)
+
+(* The core of dirac notation *)
+
+Definition bra_ket_MN (bra: Matrix 1 2) (ket : Vector 2) {n m} : Matrix (2 ^ m) (2 ^ n) := 
+  (m ⨂ ket) × (n ⨂ bra).
+Transparent bra_ket_MN. 
+
+Arguments bra_ket_MN bra ket n m /.
+
+Lemma WF_bra_ket_MN : forall n m bra ket, WF_Matrix bra -> WF_Matrix ket -> WF_Matrix (@bra_ket_MN bra ket n m).
+Proof.
+  intros.
+  unfold bra_ket_MN.
+  apply WF_mult; restore_dims; apply WF_kron_n; assumption.
+Qed.
+
+Definition Dirac_spider_semantics (bra0 bra1 : Matrix 1 2) (ket0 ket1 : Vector 2) (α : R) (n m : nat) : Matrix (2 ^ m) (2 ^ n) :=
+  (bra_ket_MN bra0 ket0) .+ (Cexp α) .* (bra_ket_MN bra1 ket1). 
+
+Arguments Dirac_spider_semantics bra0 bra1 ket0 ket1 α n m /.
+
+Lemma WF_Dirac_Spider_semantics : forall n m bra0 bra1 ket0 ket1 α, 
+                                WF_Matrix bra0 -> WF_Matrix bra1 -> WF_Matrix ket0 -> WF_Matrix ket1 -> 
+                                WF_Matrix (@Dirac_spider_semantics bra0 bra1 ket0 ket1 α n m).
+Proof.
+  intros.
+  unfold Dirac_spider_semantics.
+  apply WF_plus; restore_dims; try apply WF_scale; apply WF_bra_ket_MN; assumption.
+Qed.
+
+#[export] Hint Resolve WF_Dirac_Spider_semantics WF_bra_ket_MN : wf_db.
+
+(* Dirac semantics for a given spider *)
+
+(* TODO: Add this to QLib *)
+
+Definition braminus :=  / √ 2 .* (⟨0∣ .+ (-1 .* ⟨1∣)).
+Definition braplus  :=  / √ 2 .* (⟨0∣ .+ ⟨1∣).
+
+Notation "⟨ + ∣" := braplus.
+Notation "⟨ - ∣" := braminus.
+
+(* End TODO *)
+
+(* TODO: Move into quantum lib *)
+#[export] Hint Rewrite Mscale_kron_dist_l Mscale_kron_dist_r Mscale_mult_dist_l Mscale_mult_dist_r Mscale_assoc : scalar_move_db.
+
+Definition Z_dirac_semantics (n m : nat) (α : R) := 
+  Dirac_spider_semantics ⟨0∣ ⟨1∣ ∣0⟩ ∣1⟩ α n m.
+
+Definition X_dirac_semantics (n m : nat) (α : R) :=
+  Dirac_spider_semantics ⟨+∣ ⟨-∣ ∣+⟩ ∣-⟩ α n m.
+
+Arguments Z_dirac_semantics n m α /.
+Arguments X_dirac_semantics n m α /.
+
+Ltac unfold_dirac_spider := simpl; unfold Dirac_spider_semantics, bra_ket_MN; try (simpl; Msimpl).
+
+(** Working towards equivalence of the two forms of semantics *)
+
+Lemma ZX_Dirac_spider_X_H_Z : forall n m α, 
+  X_dirac_semantics n m α = m ⨂ hadamard × (Z_dirac_semantics n m α) × (n ⨂ hadamard).
+Proof.
+  intros.
+  simpl.
+  restore_dims.
+  rewrite Mmult_plus_distr_l.
+  rewrite Mmult_plus_distr_r.
+  apply Mplus_simplify.
+  - repeat rewrite Mmult_assoc. 
+    restore_dims.
+    rewrite kron_n_mult.
+    rewrite <- Mmult_assoc.
+    rewrite kron_n_mult.
+    replace (hadamard × ∣0⟩) with ∣+⟩ by lma.
+    replace (⟨0∣ × hadamard) with ⟨+∣ by lma.
+    reflexivity.
+  - autorewrite with scalar_move_db.
+    apply Mscale_simplify; [| lca].
+    repeat rewrite Mmult_assoc.
+    restore_dims.
+    rewrite kron_n_mult.
+    rewrite <- Mmult_assoc.
+    rewrite kron_n_mult.
+    replace (hadamard × ∣1⟩) with ∣-⟩ by lma.
+    replace (⟨1∣ × hadamard) with ⟨-∣ by lma.
+    reflexivity.
+Qed.
+
+Definition braket_0_intermediate (n m : nat) : Matrix (2^m) (2^n) :=
+  fun x y => match x, y with
+             | 0, 0 => C1
+             | _, _ => C0
+             end.
+
+Definition braket_1_intermediate (n m : nat) : Matrix (2^m) (2^n) :=
+  fun x y => if (x =? 2^m - 1) && (y =? 2^n - 1) then C1 else C0.
+
+Lemma Z_semantics_split_plus : forall (n m : nat) (α : R), Z_semantics n m α = (braket_0_intermediate n m) .+ Cexp α .* (braket_1_intermediate n m).
+Proof.
+  assert (contra : forall a, (2^S a - 1 <> 0)%nat).
+  { intros; simpl. 
+    destruct (2^a)%nat eqn:Ea. 
+    - apply Nat.pow_nonzero in Ea; [destruct Ea | easy].
+    - simpl; rewrite <- plus_n_Sm; easy.
+  } 
+  intros.
+  unfold braket_0_intermediate; unfold braket_1_intermediate.
+  unfold Z_semantics.
+  unfold Mplus, scale.
+  prep_matrix_equality.
+  destruct x, y; simpl.
+  - destruct (2^n-1)%nat eqn:En, (2^m-1)%nat eqn:Em.
+    + destruct n, m; [lca | destruct (contra m Em) | | ]; destruct (contra n En).
+    + destruct n, m; [discriminate | | | ]; lca.
+    + destruct n, m; [discriminate | | | ]; lca.
+    + destruct n, m; [discriminate | discriminate | | ]; lca.
+  - destruct (2^n-1)%nat eqn:En, (2^m-1)%nat eqn:Em.
+    + destruct n,m; [lca | destruct (contra m Em) | | ]; destruct (contra n En).
+    + destruct n, m; [discriminate | | | ]; lca.
+    + destruct n, m; [discriminate | discriminate | |]; destruct (y =? n0); lca.
+    + destruct n, m; [discriminate | | | lca]; destruct (y =? n0); lca.
+  - destruct (2^n-1)%nat eqn:En, (2^m-1)%nat eqn:Em; [lca | | lca | ]; destruct (_ =? _); lca.
+  - destruct (2^n-1)%nat eqn:En, (2^m-1)%nat eqn:Em; [lca | | lca | ]; repeat destruct (_ =? _); lca.
+Qed.
+
+
+Lemma big_bra_0_0_0 : forall n, (n ⨂ (bra 0)) 0%nat 0%nat = C1.
+Proof.
+  intros.
+  induction n; [reflexivity | ].
+  rewrite kron_n_assoc; [ | auto with wf_db].
+  unfold kron.
+  rewrite 2 Nat.div_0_l; try apply Nat.pow_nonzero; try easy.
+  rewrite 2 Nat.mod_0_l; try apply Nat.pow_nonzero; try easy.
+  rewrite IHn.
+  rewrite Cmult_1_r.
+  unfold bra.
+  unfold adjoint.
+  simpl.
+  lca.
+Qed.
+
+Lemma big_bra_S_r : forall n i j, ((S n) ⨂ bra 0) i (S j) = C0.
+Proof.
+  induction n.
+  - simpl; rewrite kron_1_l; [ | auto with wf_db ].
+    intros; unfold bra; simpl; unfold adjoint; unfold qubit0.
+    destruct i,j; lca.
+  - intros.
+    rewrite kron_n_assoc; [| auto with wf_db].
+    unfold kron.
+    destruct (S j mod 2 ^S n) eqn:En.
+    + destruct (Nat.mod_divides (S j) (2 ^ S n)); [apply Nat.pow_nonzero; auto |]. 
+      destruct (H En).
+      rewrite H1.
+      replace (2 ^ S n * x / 2 ^ S n)%nat with x.
+      * unfold bra; simpl.
+        unfold adjoint.
+        simpl.
+        destruct x.
+        -- rewrite mult_0_r in H1.
+           discriminate H1.
+        -- destruct (i / (1 ^ n + 0))%nat. 
+           ++ simpl.
+              destruct x; lca.
+           ++ simpl.
+              destruct x; lca.
+      * rewrite mult_comm.
+        rewrite Nat.divide_div_mul_exact.
+        -- rewrite Nat.div_same; [lia | ].
+           apply Nat.pow_nonzero; easy.
+        -- apply Nat.pow_nonzero; easy.
+        -- apply Nat.divide_refl.
+    + rewrite IHn.
+      lca.
+Qed.
+
+Lemma big_bra_S_l : forall n i j, (n ⨂ bra 0) (S i) j = C0.
+Proof.
+  intros.
+  assert (WF : WF_Matrix (n ⨂ bra 0)).
+  { auto with wf_db. }
+  apply WF.
+  left.
+  rewrite Nat.pow_1_l.
+  induction i; auto.
+Qed.
+
+Lemma big_ket_0_0_0 : forall n, (n ⨂ (ket 0)) 0%nat 0%nat = C1.
+Proof.
+  intros.
+  induction n; [reflexivity | ].
+  rewrite kron_n_assoc; [ | auto with wf_db].
+  unfold kron.
+  rewrite 2 Nat.div_0_l; try apply Nat.pow_nonzero; try easy.
+  rewrite 2 Nat.mod_0_l; try apply Nat.pow_nonzero; try easy.
+  rewrite IHn.
+  rewrite Cmult_1_r.
+  reflexivity.
+Qed.
+
+Lemma big_ket_S_r : forall n i j, (n ⨂ ket 0) i (S j) = C0.
+Proof.
+  intros.
+  assert (WF : WF_Matrix (n ⨂ ket 0)).
+  { auto with wf_db. }
+  apply WF.
+  right.
+  rewrite Nat.pow_1_l.
+  induction j; auto.
+Qed.
+
+Lemma big_ket_S_l : forall n i j, (S n ⨂ ket 0) (S i) j = C0.
+Proof.
+  induction n.
+  - intros. simpl.
+    rewrite kron_1_l; [ | auto with wf_db ].
+    unfold ket.
+    unfold qubit0; simpl.
+    destruct i, j;lca.
+  - intros.
+    rewrite kron_n_assoc; [ | auto with wf_db ].
+    unfold kron.
+    rewrite Nat.pow_1_l.
+    rewrite Nat.mod_1_r.
+    rewrite Nat.div_1_r.
+    destruct (S i mod 2 ^ S n) eqn:En.
+    + destruct (Nat.mod_divides (S i) (2^S n)); [apply Nat.pow_nonzero; auto |].
+      destruct H; [assumption |].
+      rewrite H.
+      rewrite mult_comm.
+      rewrite Nat.divide_div_mul_exact; [ | apply Nat.pow_nonzero; auto | apply Nat.divide_refl ].
+      rewrite Nat.div_same; [ | apply Nat.pow_nonzero; auto].
+      rewrite Nat.mul_1_r.
+      destruct x; [rewrite mult_0_r in H; discriminate H |].
+      unfold ket; simpl.
+      destruct x, j; lca.
+    + rewrite IHn.
+      lca.
+Qed.
+
+Lemma braket_sem_0_intermediate : forall (n m : nat), (n ⨂ ket 0) × (m ⨂ bra 0) = braket_0_intermediate m n.
+Proof.
+  intros.
+  destruct n,m; prep_matrix_equality.
+  - destruct x,y; lca.
+  - unfold Mmult; simpl.
+    destruct x,y; replace (m ⨂ bra 0 ⊗ bra 0) with ((S m) ⨂ bra 0) by reflexivity.
+    + rewrite big_bra_0_0_0.
+      lca.
+    + rewrite big_bra_S_r.
+      lca.
+    + rewrite big_bra_0_0_0.
+      lca.
+    + rewrite big_bra_S_r.
+      lca.
+  - unfold Mmult; rewrite Nat.pow_1_l; simpl.
+    destruct x,y; replace (n ⨂ ket 0 ⊗ ket 0) with ((S n) ⨂ ket 0) by reflexivity.
+    + rewrite big_ket_0_0_0.
+      lca.
+    + rewrite big_ket_0_0_0.
+      lca.
+    + rewrite big_ket_S_l.
+      lca.
+    + rewrite big_ket_S_l.
+      lca.
+  - unfold Mmult; rewrite Nat.pow_1_l; simpl; rewrite Cplus_0_l.
+    replace (n ⨂ ket 0 ⊗ ket 0) with ((S n) ⨂ ket 0) by reflexivity;
+    replace (m ⨂ bra 0 ⊗ bra 0) with ((S m) ⨂ bra 0) by reflexivity.
+    destruct x,y.
+    + rewrite big_ket_0_0_0; rewrite big_bra_0_0_0.
+      lca.
+    + rewrite big_bra_S_r.
+      lca.
+    + rewrite big_ket_S_l.
+      lca.
+    + rewrite big_ket_S_l.
+      lca.
+Qed.
+
+Lemma big_ket_1_max_0 : forall n, (n ⨂  ∣1⟩) (2 ^ n - 1)%nat 0%nat = C1.
+Proof.
+  induction n.
+  - lca.
+  - rewrite kron_n_assoc; [| auto with wf_db].
+    unfold kron.
+    simpl.
+    rewrite <- Nat.add_sub_assoc.
+    + replace (0 / 1 ^ n)%nat with 0%nat by (rewrite Nat.pow_1_l; rewrite Nat.div_1_r; reflexivity).
+      replace (0 mod 1^n) with 0%nat by (rewrite Nat.pow_1_l; reflexivity).
+      replace ((2 ^ n + (2 ^ n + 0 - 1)) / 2 ^ n)%nat with 1%nat.
+      * replace ((2 ^ n + (2 ^ n + 0 - 1)) mod 2 ^ n)%nat with (2^n-1)%nat.
+        -- rewrite IHn; lca.
+        -- rewrite Nat.add_mod; [| apply Nat.pow_nonzero; auto].
+           ++ rewrite plus_0_r.
+              rewrite Nat.mod_same; [| apply Nat.pow_nonzero; auto].
+              rewrite plus_0_l.
+              rewrite Nat.mod_mod; [| apply Nat.pow_nonzero; auto].
+              destruct n.
+              ** reflexivity.
+              ** rewrite Nat.mod_small; [reflexivity|].
+                 destruct (2 ^ S n)%nat eqn:E.
+                 --- destruct (Nat.pow_nonzero 2 (S n)); [auto |apply E].
+                 --- simpl.
+                     rewrite Nat.sub_0_r.
+                     constructor.
+      * rewrite plus_0_r.
+        replace ((2 ^ n + (2 ^ n - 1)) / 2 ^ n)%nat with (((1 * 2 ^ n) + (2 ^ n - 1)) / 2 ^ n)%nat.
+        -- rewrite Nat.div_add_l; [| apply Nat.pow_nonzero; auto].
+           rewrite Nat.div_small; [reflexivity|].
+           destruct (2^n)%nat eqn:E.
+           ++ destruct (Nat.pow_nonzero 2 n); [auto | apply E].
+           ++ simpl; rewrite Nat.sub_0_r.
+              auto.
+        -- rewrite mult_1_l.
+           reflexivity.
+    + rewrite plus_0_r.
+      rewrite <- (Nat.pow_1_l n).
+      replace (S (1 ^ n)) with 2%nat.
+      * apply Nat.pow_le_mono_l.
+        auto.
+      * rewrite Nat.pow_1_l; reflexivity.
+Qed.
+
+Lemma big_bra_1_0_max : forall n, (n ⨂ ⟨1∣) 0%nat (2 ^ n - 1)%nat = C1.
+Proof.
+  induction n.
+  - lca.
+  - rewrite kron_n_assoc; [| auto with wf_db].
+    unfold kron.
+    simpl.
+    rewrite <- Nat.add_sub_assoc.
+    + replace (0 / 1 ^ n)%nat with 0%nat by (rewrite Nat.pow_1_l; rewrite Nat.div_1_r; reflexivity).
+      replace (0 mod 1^n) with 0%nat by (rewrite Nat.pow_1_l; reflexivity).
+      replace ((2 ^ n + (2 ^ n + 0 - 1)) / 2 ^ n)%nat with 1%nat.
+      * replace ((2 ^ n + (2 ^ n + 0 - 1)) mod 2 ^ n)%nat with (2^n-1)%nat.
+        -- rewrite IHn; lca.
+        -- rewrite Nat.add_mod; [| apply Nat.pow_nonzero; auto].
+           ++ rewrite plus_0_r.
+              rewrite Nat.mod_same; [| apply Nat.pow_nonzero; auto].
+              rewrite plus_0_l.
+              rewrite Nat.mod_mod; [| apply Nat.pow_nonzero; auto].
+              destruct n.
+              ** reflexivity.
+              ** rewrite Nat.mod_small; [reflexivity|].
+                 destruct (2 ^ S n)%nat eqn:E.
+                 --- destruct (Nat.pow_nonzero 2 (S n)); [auto |apply E].
+                 --- simpl.
+                     rewrite Nat.sub_0_r.
+                     constructor.
+      * rewrite plus_0_r.
+        replace ((2 ^ n + (2 ^ n - 1)) / 2 ^ n)%nat with (((1 * 2 ^ n) + (2 ^ n - 1)) / 2 ^ n)%nat.
+        -- rewrite Nat.div_add_l; [| apply Nat.pow_nonzero; auto].
+           rewrite Nat.div_small; [reflexivity|].
+           destruct (2^n)%nat eqn:E.
+           ++ destruct (Nat.pow_nonzero 2 n); [auto | apply E].
+           ++ simpl; rewrite Nat.sub_0_r.
+              auto.
+        -- rewrite mult_1_l.
+           reflexivity.
+    + rewrite plus_0_r.
+      rewrite <- (Nat.pow_1_l n).
+      replace (S (1 ^ n)) with 2%nat.
+      * apply Nat.pow_le_mono_l.
+        auto.
+      * rewrite Nat.pow_1_l; reflexivity.
+Qed.
+
+Lemma big_ket_1_n_S : forall n i j, (n ⨂  ∣1⟩) i (S j) = C0.
+Proof.
+  induction n.
+  - intros.
+    simpl.
+    destruct i.
+    + lca.
+    + unfold I.
+      replace (S i <? 1) with false; [| reflexivity].
+      rewrite andb_false_r.
+      reflexivity.
+  - intros.
+    simpl.
+    unfold kron.
+    rewrite Nat.div_1_r.
+    rewrite IHn.
+    lca.
+Qed.
+
+Definition big_bra_sem (n : nat) : Matrix 1 (2 ^ n) :=
+  fun x y => 
+  if (y =? 2^n-1) && (x =? 0) then C1 else C0.
+
+Opaque Nat.div.
+Opaque Nat.modulo.
+
+Lemma big_bra_to_sem : forall n, (n ⨂ (bra 1)) = big_bra_sem n.
+Proof.
+  induction n.
+  - prep_matrix_equality.
+    destruct x,y.
+    + lca.
+    + lca.
+    + lca.
+    + unfold big_bra_sem.
+      rewrite andb_false_r.
+      simpl.
+      unfold I.
+      rewrite andb_false_r.
+      reflexivity.
+  - prep_matrix_equality.
+    simpl.
+    rewrite IHn.
+    unfold kron.
+    destruct (y =? 2^(S n) - 1) eqn:Ex.
+    + unfold big_bra_sem.
+      rewrite Ex.
+      apply Nat.eqb_eq in Ex.
+      rewrite Ex.
+      rewrite Nat.mod_1_r.
+      rewrite Nat.div_1_r.
+      destruct y.
+      * destruct (2^n)%nat eqn:En.
+        -- contradict En.
+           apply Nat.pow_nonzero.
+           easy.
+        -- replace ((2 ^ S n - 1) / 2)%nat with (2^n - 1)%nat.
+           ++ rewrite En.
+              rewrite Nat.eqb_refl.
+              replace ((2 ^ S n - 1) mod 2)%nat with 1%nat.
+              ** destruct x; lca.
+              ** replace (2 ^ S n)%nat with (2^n + 2^n)%nat.
+                 --- destruct (2 ^ n)%nat eqn:E2n.
+                     +++ contradict E2n.
+                         apply Nat.pow_nonzero; easy.
+                     +++ rewrite <- plus_n_Sm.
+                         replace (S (S n1 + n1) - 1)%nat with (S (n1 + n1))%nat by reflexivity.
+                         rewrite (double_mult n1).
+                         rewrite <- (plus_0_l (2*n1)).
+                         replace (S (0 + 2 * n1))%nat with (1 + 2 * n1)%nat by reflexivity.
+                         rewrite Nat.add_mod; [| easy].
+                         rewrite mult_comm.
+                         rewrite Nat.mod_mul; [| easy].
+                         reflexivity.
+                 --- simpl.
+                     rewrite plus_0_r.
+                     lia.
+           ++ replace (2 ^ S n)%nat with (2 * (2 ^ n))%nat.
+              ** destruct (2^n)%nat.
+                 --- reflexivity.
+                 --- contradict Ex.
+                     destruct (2^S n)%nat eqn:Esn.
+                     +++ contradict Esn.
+                         apply Nat.pow_nonzero; easy.
+                     +++ destruct n2.
+                         *** contradict Esn.
+                             simpl.
+                             destruct (2^n)%nat.
+                             ---- easy.
+                             ---- destruct n2.
+                                  ++++ easy.
+                                  ++++ simpl.
+                                       easy.
+                         *** easy.
+              ** reflexivity.
+      * Opaque Nat.div.
+        Opaque Nat.modulo.
+        replace ((2 ^ S n - 1) / 2)%nat with (2^n - 1)%nat.
+        replace ((2 ^ S n - 1) mod 2)%nat with 1%nat.
+        -- rewrite Nat.eqb_refl.
+           destruct x; lca.
+        -- simpl.
+           rewrite plus_0_r.
+           destruct (2 ^ n)%nat eqn:En.
+           ++ contradict En.
+              ** apply Nat.pow_nonzero; easy.
+           ++ simpl.
+              rewrite <- plus_n_Sm.
+              rewrite Nat.sub_0_r.
+              rewrite double_mult.
+              replace (S (2 * n0))%nat with (1 + (2 * n0))%nat by reflexivity.
+              rewrite mult_comm.
+              rewrite Nat.add_mod; [| easy].
+              rewrite Nat.mod_mul; [| easy].
+              reflexivity.
+        -- simpl.
+           rewrite plus_0_r.
+           destruct (2 ^ n)%nat.
+           ++ reflexivity.
+           ++ simpl.
+              rewrite Nat.sub_0_r.
+              rewrite Nat.sub_0_r.
+              rewrite <- plus_n_Sm.
+              rewrite double_mult.
+              replace (S (2 * n0))%nat with ((1 + (2 * n0)))%nat by reflexivity.
+              rewrite plus_comm.
+              rewrite mult_comm.
+              rewrite Nat.div_add_l; [| easy].
+              rewrite plus_comm.
+              reflexivity.
+    + unfold big_bra_sem.
+      rewrite Ex.
+      simpl.
+      rewrite Nat.mod_1_r.
+      Transparent Nat.div.
+      destruct (Nat.divmod y 1 0 1) eqn:Edm.
+      assert (Hy : (y = 2 * (y / 2) + y mod 2)%nat).
+      { apply Nat.div_mod; lia. } (* Nat.div_mod_eq works in 8.14 on *)
+      destruct (y/2 =? 2^n-1) eqn:Ey2.
+      * destruct (y mod 2 =? 1) eqn:Eym.
+        -- apply Nat.eqb_eq in Eym, Ey2.
+           rewrite Ey2, Eym in Hy.
+           replace (2 * (2 ^ n - 1) + 1)%nat with (2 ^ S n - 1)%nat in Hy.
+           ++ rewrite Hy in Ex.
+              rewrite Nat.eqb_refl in Ex.
+              discriminate.
+           ++ simpl.
+              rewrite 2 plus_0_r.
+              rewrite <- plus_assoc.
+              rewrite <- plus_n_Sm.
+              rewrite plus_0_r.
+              destruct (2 ^ n)%nat eqn:En.
+              ** contradict En.
+                 apply Nat.pow_nonzero; easy.
+              ** simpl. lia.
+        -- destruct (y mod 2).
+           ++ lca.
+           ++ destruct n2.
+              ** discriminate.
+              ** lca.
+      * lca.
+Qed.
+
+Definition big_ket_sem (n : nat) : Matrix (2 ^ n) 1 :=
+  fun x y => 
+  if (x =? 2^n-1) && (y =? 0) then C1 else C0.
+
+Lemma big_ket_sem_big_bra_sem_transpose : forall n, big_ket_sem n = (big_bra_sem n) ⊤.
+Proof.
+  intros.
+  unfold big_ket_sem, big_bra_sem.
+  unfold transpose.
+  reflexivity.
+Qed.
+
+Lemma big_ket_to_sem : forall n, (n ⨂ (ket 1)) = big_ket_sem n.
+Proof.
+  intros.
+  rewrite <- (transpose_involutive _ _ _).
+  rewrite kron_n_transpose.
+  replace ((ket 1)⊤) with (bra 1).
+  - rewrite big_ket_sem_big_bra_sem_transpose.
+    f_equal.
+    + rewrite Nat.pow_1_l.
+      easy.
+    + apply big_bra_to_sem.
+  - rewrite ket1_transpose_bra1.
+    reflexivity.
+Qed.
+
+Lemma braket_sem_1_intermediate : forall n m : nat, n ⨂ ket 1 × m ⨂ bra 1 = braket_1_intermediate m n.
+Proof.
+  intros.
+  rewrite big_bra_to_sem.
+  rewrite big_ket_to_sem.
+  prep_matrix_equality.
+  unfold braket_1_intermediate, big_ket_sem, big_bra_sem, Mmult.
+  rewrite Nat.pow_1_l; simpl.
+  rewrite Cplus_0_l.
+  destruct (x =? 2^n-1), (y =? 2^m-1); lca.
+Qed.
+
+Lemma Z_semantics_equiv : forall n m α, Z_semantics n m α = Z_dirac_semantics n m α.
+Proof.
+  intros.
+  simpl.
+  replace (m ⨂ ∣0⟩ × n ⨂ ⟨0∣)
+     with (braket_0_intermediate n m).
+  replace (m ⨂ ∣1⟩ × n ⨂ ⟨1∣)
+     with (braket_1_intermediate n m).
+  apply Z_semantics_split_plus.
+  rewrite braket_sem_1_intermediate; auto.
+  rewrite braket_sem_0_intermediate; auto.
+Qed.
+
+Lemma X_semantics_equiv : forall n m α, X_semantics n m α = X_dirac_semantics n m α.
+Proof.
+  intros.
+  rewrite ZX_Dirac_spider_X_H_Z.
+  unfold X_semantics.
+  Msimpl.
+  restore_dims.
+  rewrite Z_semantics_equiv.
+  reflexivity.
+Qed.
+
+Lemma WF_Z_semantics : forall n m α, WF_Matrix (Z_semantics n m α).
+Proof. intros; rewrite Z_semantics_equiv; apply WF_Dirac_Spider_semantics; auto with wf_db. Qed.
+
+Lemma WF_X_semantics : forall n m α, WF_Matrix (X_semantics n m α).
+Proof. intros; rewrite X_semantics_equiv; apply WF_Dirac_Spider_semantics; 
+       unfold braplus, braminus; auto with wf_db. Qed.
+
+#[export] Hint Resolve WF_Z_semantics WF_X_semantics : wf_db.
+
